\begin{exercise}
	Let $P$ be a graded poset, $M$ a special matching, and $x\in P$ such that $M(x)\lessdot x$. Prove that $M$ restrict to special matching of $\{y\in P: y\leq x\}$.
\end{exercise}

\begin{exercise}
	Let $v\in \mathfrak{S}_n$ and $M,M'$ be two special matchings on $[1,v]$ such that $M(u)=M'(u)$ for $\ell(u)\leq 1$. Prove that $M=M'$. (Q: Is this true for other types?)
\end{exercise}

\begin{theorem}
	Diamonds?
\end{theorem}

\section{Kazhdan-Lusztig Polynomials}
\begin{definition}
	Define a map $\eta$ by
	\begin{align*}
	\eta:\mathbb{Z}[q,q^{-1}]&\to\mathbb{Z}[q,q^{-1}]\\
	q&\mapsto q^{-1}
	\end{align*}

Let $\eta(T_w)=\mapsto (T_{w^{-1}})^{-1}$ and extend by linearity to $H(q)$.
\end{definition}
\begin{prop}
	$\eta^2(T_s)=T_s$
\end{prop}
\begin{proof}$\eta^2(T_s)=\eta(q^{-1}T_s-(1-q^{-1})T_1)=T_s-(q-1)T_1-(1-q)T_1=T_s
$
\end{proof}
\begin{theorem}
	$\eta$ is a ring homomorphism.
\end{theorem}
\begin{proof}
	We first prove that $\eta(T_wT_s)=\eta(T_w)\eta(T_s)$.
	
	\paragraph{Case (1) $\ell(sw)>\ell(w)$}
	\[\eta(T_sT_w)=\eta(T_{sw})=T^{-1}_{(sw)^{-1}}=\left(T_{w^{-1}s}\right)^{-1}=\left(T_{w^{-1}}T_s\right)^{-1}=T_s^{-1}T_{w^{-1}}^{-1}=\eta(T_s)\eta(T_w)\]
	\paragraph{Case (2) $\ell(sw)<\ell(w)$} Let $v=w^{-1}s$.
	\begin{align*}
	\eta(T_sT_w)&=\eta(qT_{sw}+(q-1)T_w)=q^{-1}\left(T_{(sw)^{-1}}\right)^{-1}+(q^{-1}-1)T_{w^{-1}}^{-1}=q^{-1}T_v^{-1}+(q^{-1}-1) T_{w^{-1}}^{-1}
	\end{align*}
	\[T_{w^{-1}}=T_{vs}=T_vT_s\implies \left(T_{w^{-1}}\right)^{-1}=T_s^{-1}T_v^{-1}=\left(q^{-1}T_s-(1-q^{-1})T_1\right)T_v^{-1}\]
	Putting these together:
	\begin{align*}\eta(T_sT_s)&=q^{-1}T_v^{-1}+(q^{-1}-1)q^{-1}T_sT_v^{-1}-(q^{-1}-1)(1-q^{-1})T_v^{-1}\\
	&=(-q^{-1}+q^{-2}+1)T_v^{-1}-q^{-2}(q-1)T_sT_v^{-1}\end{align*}
	Now calculate
	\[\eta(T_s)\eta(T_w)=T_s^{-1}(T_{w^{-1}})^{-1}=T_s^{-2}T_v^{-1}\]
	where
	\begin{align*}T_s^{-2}&=(q^{-1}T_s-(1-q^{-1})T_1)^{2}=q^{-2}T_s^2-2q^{-1}(1-q^{-1})T_s+(1-q^{-1})^2T_1\\
	&=q^{-2}((q-1)T_s+qT_1)-2q^{-1}(1-q^{-1})T_s+(1-q^{-1})^{-2}T_1\\
	&=(-q^{-2}(q-1))T_s+(1-q^{-1}+q^{-2})T_1
	\end{align*}
	Comparing we get that $\eta(T_sT_w)=\eta(T_s)\eta(T_w)$.
	
	In general we need to show that $\eta(T_{w'}T_w)=\eta(T_{w'})\eta(T_w)$. We induct on length $\ell(w')$.
	\begin{align*}
		\eta(T_{w'}T_w)&=\eta(T_{w's}T_sT_w)
		=\eta(T_{w's})\eta(T_sT_w)\\&=\eta(T_{w's})\eta(T_s)\eta(T_w)=\eta(T_{w's})T_s)\eta(T_w)=\eta(T_{w'})\eta(T_w)\qedhere
	\end{align*}

	

\end{proof}