\documentclass[12pt]{amsart}
\usepackage{mathptmx}
\usepackage{stmaryrd}
\usepackage{amssymb}
\usepackage{mathtools}
\include{command}
\numberwithin{equation}{section}
\usepackage{xcolor}
\usepackage{ytableau}
%\include{theorems}

\newcommand{\llb}[0]{\llbracket}
\newcommand{\rrb}[0]{\rrbracket}
\newlength\friezelen 
\settowidth{\friezelen}{$\xi_{m}$} % calculate width of widest element

\usepackage{array} % for "\newcolumntype" macro
\newcolumntype{Q}{>{\centering}p{\friezelen}<{}}


\usepackage{mathtools}
\usepackage{verbatim}
\usepackage{comment}
\usetikzlibrary{arrows}
\tikzset {->-/.style={decoration={markings, mark=at position .5 with {\arrow{latex}}}, postaction={decorate}}}
\tikzset {-->-/.style={decoration={markings, mark=at position .5 with {\arrow[scale=2]{latex}}}, postaction={decorate}}}
\newcommand{\midarrow}{\tikz \draw[-triangle 90] (0,0) -- +(.1,0);}
\newcommand{\miduparrow}{\tikz \draw[-triangle 90] (0,0) -- +(.1,0);}
\newcommand{\midrevarrow}{\tikz \draw[-triangle 90] (0,0) -- +(-.1,0);}
\usepackage{comment}
%\usepackage{graphicx}
\usepackage{color}
\usepackage{etoolbox}
\usepackage[margin=1in]{geometry}
%\usepackage{amsmath,amsthm,amssymb,graphicx,tikz,tikz-cd}
\usepackage{hyperref}
\hypersetup{
    colorlinks = true,
    citecolor = orange,%
}
\usepackage[noabbrev]{cleveref}
\usepackage{subcaption}

\makeatletter
\patchcmd{\@settitle}{\uppercasenonmath\@title}{}{}{}
\patchcmd{\@setauthors}{\MakeUppercase}{}{}{}
\patchcmd{\section}{\scshape}{}{}{}
\makeatother
\makeatletter
\patchcmd{\@maketitle}
  {\ifx\@empty\@dedicatory}
  {\ifx\@empty\@date \else {\vskip2ex %vertical position of date
  \centering\footnotesize\@date\par\vskip1ex}\fi
   \ifx\@empty\@dedicatory}
  {}{}
\patchcmd{\@adminfootnotes}
  {\ifx\@empty\@date\else \@footnotetext{\@setdate}\fi}
  {}{}{}
\makeatother


\renewcommand{\l}[2]{\lambda_{#1,#2}}
\newcommand{\ls}[0]{\prescript{*}{}}
\newcommand{\cal}[1]{\mathcal{#1}}

\theoremstyle{plain}
\newtheorem{theorem}{Theorem}[section]
\newtheorem{restate}{Theorem}[section]
\newtheorem{lemma}[theorem]{Lemma}
\newtheorem{prop}[theorem]{Proposition}
\newtheorem{conj}[theorem]{Conjecture}
\newtheorem{question}[theorem]{Question}
\newtheorem{corollary}[theorem]{Corollary}
\newtheorem{claim}[theorem]{Claim}
\theoremstyle{definition}
\newtheorem{remark}[theorem]{Remark}
\newtheorem{example}[theorem]{Example}
\newtheorem{definition}[theorem]{Definition}
\newtheorem{exercise}[theorem]{Exercise}


\newcommand{\todo}[1]{{\color{red}[To Do: #1]}}
\newcommand{\syl}[1]{{\color{orange}[Sylvester: #1]}}
\newcommand{\new}[1]{{#1}}
\newcommand{\calG}[0]{\mathcal{G}}
\newcommand{\sn}[0]{\mathfrak{S}_n}
\DeclareMathOperator{\mani}{\textbf{Man}}
\DeclareMathOperator{\s}{\textbf{S}}
\DeclareMathOperator{\sgn}{sgn}

\title{Topics in Combinatorics: Kazhdan-Lusztig Theory}
%\author{Sylvester W. Zhang}

\thanks{School of Mathematics, University of Minnesota, Minneapolis, MN 55455, USA}
\thanks{\emph{Email}:
\href{mailto:swzhang@umn.edu}{swzhang@umn.edu}}
\thanks{Last updated: \today}
\begin{document}


\maketitle
\begin{abstract}
	Topics course in combinatorics at University of Minnesota (\href{https://sites.google.com/view/8680spring2023/home}{MATH 8680}) taught by Prof. Pavlo Pylyavskyy.
\end{abstract}
\setcounter{tocdepth}{1}
\tableofcontents
\setlength{\parindent}{0em}
\setlength{\parskip}{0.618em}

\tableofcontents
\input{jan18.tex}



\section{Basics of Coxeter Groups and Hecke Algebras}
\begin{theorem}\label{thm:Hecke}
	
\end{theorem}
The most technical step of proving this theorem if the following lemma, whose proof we defer after proving \Cref{thm:Hecke}
\begin{lemma}\label{lem:lam_rho_commute}
	$\lambda$ and $\rho$'s commute.
\end{lemma}

\begin{lemma}
	$\varphi$ is surjective.
\end{lemma}
\begin{lemma}
	$\varphi$ is injective.
\end{lemma}
\begin{proof}{proof of \Cref{thm:Hecke}}
	Need to check the relations.
	1) $\lambda_s\lambda_w=\lambda_{sw}$ if $sw>w$. This is true by definition.
	
	2) Need to show that $\lambda_s^2 = a_s \lambda_s+b_s\lambda_1$. Now take any basis element of the vector space $\mathcal{E}$, $T_w$, need to show that
	\[\lambda_s^2T_w = a_s\lambda_s T_2 + b_s\lambda_1 T_w\]
	for any $w$.
	If $\ell(sw)>\ell(w)$,
	\[\lambda_s(\lambda_s T_w)=\lambda_s(T_{sw})=a_sT_{sw}+bs T_w=(a_s\lambda_s+b_s\lambda_1)T_w\]
	If $sw<w$, then
	\[\lambda_s^2(T_w)=\lambda_2(a_sT_w+b_sT_{sw})=a_s\lambda_s T_w+b_s\underbrace{\lambda_s T_{sw}}_{=T_{ssw}=T_w}=a_s\lambda_sT_w+b_s\lambda_1 T_w\qedhere\]
\end{proof}
We are left to prove \Cref{lem:lam_rho_commute}, before doing that we need another lemma.

\begin{lemma}
	Let $w\in W$ and $s,t\in S$. If $\ell(swt)=\ell(w)$ and $\ell(sw)=\ell(wt)$, then $sw=wt$.
\end{lemma}
\begin{proof}
	Assume $w=s_1\cdots s_r$ reduced. If $\ell(sw)>\ell(w)$, then $\ell(w)=\ell(swt)<\ell(sw)$, which implies that $sw=w't$, where $w'=w$ or $s s_1\cdots \hat s_i\cdots s_r=w'$.
	
	\[wt=s\cdot swt=s\cdot w't t=sw'=s_1\cdots \hat{s_i}\cdots s_r\implies \ell(wt)\neq \ell(sw)\]
\end{proof}
We are now ready to prove \Cref{lem:lam_rho_commute}.
\begin{proof}[Proof of \Cref{lem:lam_rho_commute}]Consider the following cases.
	
	a) $\ell(w)=\ell(wt)=\ell(sw)<\ell(swt)$
	\todo{Make some pictures to illustrate the cases}
	\[\lambda_s\rho_t(T_w)=\lambda_s(T_{wt})=T_{swt}\]
	\[\rho_t\lambda_s(T_w)=\rho_t(T_{sw})=T_{swt}\]
	b) $\ell(swt)=\ell(w)<\ell(wt)=\ell(sw)$. By lemma $sw=wt$.
	\[\lambda_s\rho_t(T_w)=\lambda_s(T_{wt})=a_sT_{wt}+b_sT_{swt}\]
	\[\rho_t\lambda_s(T_w)=\rho_t(T_{sw})=a_tT_{sw}+b_tT_{swt}\]
	
	c) $\ell(swt)<\ell(sw)=\ell(wt)<\ell(w)$
	\[\lambda_s\rho_t(T_w) \lambda_s(a_t T_w+b_t T_{wt}=a_t a_s T_w+a_t b_s T_{sw} +b_t a_s T_{wt} +b_t b_s T_{sw} \]
	Can check that $\rho_t \lambda_s(T_w)$ gives the same result.
	
	d)$\ell(wt)=\ell(sw)<\ell(w)=\ell(swt)$. By previous lemma, we have $sw=wt$.
	\[ \lambda_s\rho_t(T_w)=\lambda_s(a_tT_w+b_t T_{wt})=a_ta_sT_w+a_tb_sT_{sw}+b_t T_{swt} \]
	\[\rho_t\lambda_t(T_w)=\rho_t(a_s T_w+b_s T_{sw})=a_sa_tT_w+a_sb_tT_{wt}+b_sT_{swt}\]
	
	e) $\ell(wt)<\ell(w)=\ell(swt)<\ell(sw)$.
	\[\lambda_s\rho_t(T_w)=\lambda_s(a_t T_w+b_tT_{wt})=a_t T_{sw}+b_tT_{swt}\]
	\[\rho_t \lambda_s(T_w)=\rho_t(T_{sw})=a_t T_{sw}+b_t T_{swt}=\cdots \cdots\] 
\end{proof}
\todo{Need to finish.}
\section{$R$-polynomials}
From now on we will work in the case of Hecke algebras with equal parameters, i.e. $a_s=q-1,b_s=q$. In other words, out Hecke algebra relations will be
\[\begin{cases}
	T_sT_w=T_{sw}&sw>w\\
	T_s^2=(q-1)T_s+qT_1
\end{cases}\]
Note that $T_s$ is invertible for all $s\in S$:
\[T_s^{-1}=q^{-1}T_s-(1-q^{-1})T_1.\]
Note that this implies that all $T_w$ are invertible. In particular, we can write down the explicit formula for $T_{w^{-1}}^{-1}$, which will be a combination of $T_x$ for $x\leq w$. This leads to the definition of $R$-polynomials.


\begin{theorem}\label{thm:def_R_poly}
Denote $\varepsilon_w =(-1)^{\ell(w)}$ and $q_w=q^{\ell(w)}$. We have
\[\left(T_{w^{-1}}\right)^{-1}=\varepsilon_w q_w^{-1}\sum_{x\leq w}\varepsilon_x R_{x,w}(q),\]
where $R_{x,w}(q)\in\mathbb{Z}[q]$ is a polynomial of degree $\ell(x,w):=\ell(w)-\ell(u)$. Note that $R_{w,w}=1$.
\end{theorem}
\begin{example}If $w=s\in S$, we have
	\[T_{s}^{-1}=-q^{-1}\left( -R_{s,s}(q)T_s+R_{1,s}(q)T_1\right).\]
	This has to be equal to $q^{-1}T_s-(1-q^{-1})T_1$. By matching up coefficients we get
	\[R_{s,s}(q)=1,\quad R_{1,s}(q)=q-1.\]
\end{example}
\begin{example}
	Consider $A_1$ with $2$ generators $S=\{s,t\}$, and let $w=st$.
	\begin{align*}
		T_{(st)^{-1}}^{-1}&=T_{ts}^{-1}=T_s^{-1}T_t^{-1}\\&=\left(q^{-1}T_s-(1-q^{-1})T_1\right)\cdot\left(q^{-1}T_t-(1-q^{-1})T_1\right)\\
		&=q^{-2}\left(T_{st}-(q-1)T_s-(q-1)T_t+(q-1)^2T_1\right)
	\end{align*}
	From here we see that
	\[R_{st,st}=1,\ R_{s,st}=q-1,\ R_{t,st}=q-1,\ R_{1,st}=(q-1)^2\]
\end{example}
\begin{example}
	Similar to the previous but this time we take $w=sts$.
	\begin{align*}
		T_{(sts)^{-1}}^{-1}&=T_s^{-1}T_t^{-1}T_s^{-1}\\
		&=q^{-3}(T_s-(q-1)T_1)\cdot(T_t-(q-1)T_1)\cdot(T_s-(q-1)T_1)\\
		&=q^{-3}\big[T_{sts}-(q-1)T_{ts}-(q-1)T_{st}-(q-1)T_s^2+2(q-1)^2T_s+(q-1)^2T_t-(q-1)^3T_1\big]\\
		&=q^{-3}\big[T_{sts}-(q-1)T_{ts}-(q-1)T_{st}+(q-1)^2 T_s+(q-1)^2T_t-(q^3-2q^2+2q-1)T_1\big]
	\end{align*}
	From this we conclude
	\[R_{sts,sts}=1,\ R_{st,sts}=R_{ts,sts}=q-1\, R_{t,sts}=R_{s,sts}=(q-1)^2,\ R_{1,sts}=q^3-2q^2+2q-1\]
\end{example}
\begin{conj}\label{conj:comb_inv}
	In any Coxeter group $W$, $R_{x,w}(q)$ only depends on the isomorphism type of the Bruhat interval $[x,w]$.
\end{conj}
\begin{remark}
	\Cref{conj:comb_inv} is know to be true in type $A_{n-1}$ [Cite], and in the case when $[x,w]$ has a special matching [cite].
\end{remark}

\begin{lemma}
	Let $s\in S,w\in W$ such that $sw<w$. Assume that $x<w$, then
	\begin{enumerate}[]
		\item if $sx<x$, then $sx<sw$.
		\item if $sx>x$, then $sx\leq w,x\leq sw$
	\end{enumerate}
\end{lemma}
\begin{proof}
	Proof is a little bit painful :( so will be omitted :)
\end{proof}

\input{feb01.tex}
\input{feb03.tex}
\input{feb06.tex}
\input{feb08.tex}
\input{feb10.tex}
\input{feb13.tex}
\input{feb15.tex}
\input{feb17.tex}
\input{feb20.tex}
\input{feb22.tex}
\input{feb24.tex}
\input{feb27.tex}
\input{mar13.tex}
\input{mar15.tex}
\input{mar22.tex}
\input{mar24.tex}

\bibliographystyle{alpha}
\bibliography{main}
\end{document}


\end{document}